Book.thy
@@ -1229,10 +1229,20 @@ lemma dreg_before_step:
   shows "i \<in> Step_class \<mu> l k {dreg_step}"
   using assms by (auto simp: Step_class_def stepper_kind_def split: if_split_asm prod.split_asm)
 
+lemma dreg_before_step':
+  assumes "i \<in> Step_class \<mu> l k {red_step,bblue_step,dboost_step}" "i>0"
+  shows "i - Suc 0 \<in> Step_class \<mu> l k {dreg_step}"
+  by (simp add: assms dreg_before_step)
+
 lemma step_before_freg:
   assumes "Suc i \<in> Step_class \<mu> l k {dreg_step}"
   shows "i \<in> Step_class \<mu> l k {red_step,bblue_step,dboost_step}"
   using assms by (auto simp: step_kind_defs split: if_split_asm prod.split_asm)
+
+lemma step_before_freg':
+  assumes "i \<in> Step_class \<mu> l k {dreg_step}" "i>0"
+  shows "i - Suc 0\<in> Step_class \<mu> l k {red_step,bblue_step,dboost_step}"
+  by (simp add: assms step_before_freg)
 
 lemma step_odd: "i \<in> Step_class \<mu> l k {red_step,bblue_step,dboost_step} \<Longrightarrow> odd i" 
   by (auto simp: Step_class_def stepper_kind_def split: if_split_asm prod.split_asm)
